Add a little more to the wal invariant

src/program_proof/wal/proof.v
@@ -5,6 +5,7 @@ From Perennial.program_proof Require Import wal.circular_proof.
 
 Definition LogPositionT := wal.LogPosition.
 Definition LogPosition := u64.
+Definition LogDiskBlocks := 513.
 
 Class ToVal {ext:ext_op} {ext_ty: ext_types ext} T (t: @ty val_tys) :=
   { to_val : T → val;
@@ -53,22 +54,50 @@ End WalogM.
 Section heap.
 Context `{!heapG Σ}.
 Context `{!lockG Σ}.
+Implicit Types (Φ: val → iProp Σ).
 Implicit Types (v:val) (z:Z).
+
+Theorem post_upto_intval Φ (x1 x2: u64) :
+  int.val x1 = int.val x2 →
+  Φ #x1 -∗ Φ #x2.
+Proof.
+  iIntros (Heq%word.unsigned_inj) "HΦ".
+  subst; auto.
+Qed.
+
+Theorem LogDiskBlocks_ok Φ :
+  Φ #LogDiskBlocks -∗ WP LOGDISKBLOCKS {{ Φ }}.
+Proof.
+  iIntros "HΦ".
+  rewrite /LOGDISKBLOCKS /HDRADDRS.
+  wp_pures.
+  iApply "HΦ".
+Qed.
+
+Opaque u64_instance.u64.
 
 Definition walN: namespace := nroot .@ "wal".
 
 Definition lockInv (l: loc) (σ: log_state.t): iProp Σ :=
   (∃ memLog diskLog
      (memStart: u64) (diskStart: u64) (nextDiskEnd: u64)
-     memLogCache,
-      (is_circular (l +ₗ 2) (circΣ.mk diskLog diskStart)) ∗
+     memLogCache
+     (installedDisk: disk),
+      let log_σ := circΣ.mk diskLog diskStart in
+      (* these are the real positions; the abstract state lags them *)
+      let durable_to := circΣ.diskEnd log_σ in
+      let installed_to := diskStart in
+      (is_circular (l +ₗ 2) log_σ) ∗
       (∃ s, (l +ₗ 5) ↦[slice.T (struct.t Update.S)] (slice_val s) ∗
       updates_slice s memLog) ∗
       (l +ₗ 7) ↦[uint64T] #memStart ∗
       (l +ₗ 8) ↦[uint64T] #nextDiskEnd ∗
       is_map (l +ₗ 12) memLogCache ∗
       ⌜int.val memStart ≤ int.val diskStart⌝ ∗
-      ⌜∃ memLog', memLog = diskLog ++ memLog'⌝
+      ⌜∃ memLog', memLog = diskLog ++ memLog'⌝ ∗
+      ⌜int.val σ.(log_state.durable_to) <= int.val durable_to⌝ ∗
+      ⌜int.val σ.(log_state.installed_to) <= int.val installed_to⌝ ∗
+      [∗ map] a↦b ∈ installedDisk, LogDiskBlocks d↦ b
   ).
 
 Definition is_wal (l: loc) (σ: log_state.t): iProp Σ :=
